updating

coq/Relation.v
@@ -2,5 +2,5 @@ Definition relation (X: Type) : Type := X -> X -> Prop.
 
 Inductive multi {X : Type} (R : relation X) : relation X :=
   | multi_base : forall (x y : X), R x y -> multi R x y
-  | multi_step : forall (x y z : X), multi R x y -> R y z -> multi R x z
+  | multi_trans : forall (x y z : X), multi R x y -> R y z -> multi R x z
 .
